Now supports declaration of external functions (aka code-printing setup)

regression/src/test_external_fun.c
@@ -1,0 +1,16 @@
+#include <stdio.h>
+#include <stdint.h>
+#include <assert.h>
+
+#include "test_external_fun.h"
+
+uint64_t external_fun(uint64_t n) {
+  return n+1;
+}
+
+
+int main(int argc, char **argv) {
+  assert (uses_external_fun(42) == 44);
+  
+  return 0;
+}
